temporary result

src/simple-proof/alg-proof/InvertibleTyping.v
@@ -1,6 +1,6 @@
 Require Import Definitions TightTyping.
 Require Import InertTypes.
-
+  
 
 Reserved Notation "G '⊢##' x '⦂' T" (at level 70, T at level 79).
 
@@ -23,23 +23,14 @@ Inductive ty_var_inv : env -> atom -> typ -> Prop :=
     G ⊢## x ⦂ μ{ DS1 } ->
     G ⊢## x ⦂ μ{ DS2 } ->
     G ⊢## x ⦂ μ{ append DS1 DS2 }
-| ty_obj_fld_inv : forall L G x a T (DS1 DS2 : decs) U,
+| ty_obj_fld_inv : forall G x a T (DS1 DS2 : decs) U,
     G ⊢## x ⦂ μ{ append DS1 $ decs_cons (label_trm a) (dec_trm T) DS2 } ->
-    (forall x, x `notin` L ->
-          x ~ open_typ_to_context x
-            (μ{ append DS1 $ decs_cons (label_trm a) (dec_trm T) DS2 }) ++
-            G ⊢ T <⦂ U) ->
+    G ⊢# T <⦂ U ->
     G ⊢## x ⦂ μ{ append DS1 $ decs_cons (label_trm a) (dec_trm U) DS2 }
-| ty_obj_typ_inv : forall L G x A (DS1 DS2 : decs) S1 T1 S2 T2,
+| ty_obj_typ_inv : forall G x A (DS1 DS2 : decs) S1 T1 S2 T2,
     G ⊢## x ⦂ μ{ append DS1 $ decs_cons (label_typ A) (dec_typ S1 T1) DS2 } ->
-    (forall x, x `notin` L ->
-          x ~ open_typ_to_context x
-            (μ{ append DS1 $ decs_cons (label_typ A) (dec_typ S1 T1) DS2 }) ++
-            G ⊢ S2 <⦂ S1) ->
-    (forall y, y `notin` L ->
-          y ~ open_typ_to_context y
-            (μ{ append DS1 $ decs_cons (label_typ A) (dec_typ S1 T1) DS2 }) ++
-            G ⊢ T1 <⦂ T2) ->
+    G ⊢# S2 <⦂ S1 ->
+    G ⊢# T1 <⦂ T2 ->
     G ⊢## x ⦂ μ{ append DS1 $ decs_cons (label_typ A) (dec_typ S2 T2) DS2 }
 | ty_obj_sel_inv : forall G x y DS S A,
     G ⊢## x ⦂ S ->
@@ -50,7 +41,7 @@ Inductive ty_var_inv : env -> atom -> typ -> Prop :=
     G ⊢## x ⦂ all(S1) T1 ->
     G ⊢# S2 <⦂ S1 ->
     (forall x, x `notin` L ->
-       x ~ S1 ++ G ⊢ open x T1 <⦂ open x T2) ->
+       x ~ S2 ++ G ⊢ open x T1 <⦂ open x T2) ->
     G ⊢## x ⦂ all(S2) T2
 | ty_top_inv : forall G x T,
     G ⊢## x ⦂ T ->
@@ -94,6 +85,25 @@ Lemma invertible_typing_closure_tight: forall G x T U,
     G ⊢# T <⦂ U ->
     G ⊢## x ⦂ U.
 Proof.
+  induction on subtypt; eroutine.
+  (* all:inv typing undec 1; *)
+  (*   eprove from inert at 6. *)
+  prove from inert.
+  Focus 3.
+  prove from inert.
+  Focus 3.
+  eprove from inert at 6.
+  Focus 3.
+  invert H4; prove from inert.
+
+  eapply ty_obj_fld_inv. eassumption.
+  
+  eprove from inert at 6.
+  prove from inert.
+  eprove from inert at 6.
+  eprove from inert.
+  all: inv typing undec 1.
+  prove from inert.
   induction on subtypt; eroutine;
     inv typing undec 1;
     eprove from inert at 6.
@@ -108,7 +118,219 @@ Proof.
   eapply invertible_typing_closure_tight; try eassumption.
   eauto.
 Qed.
+
+
+Lemma inert_subtyp_obj : forall G x DS L D,
+    inert_env G ->
+    G ⊢## x ⦂ μ{ DS } ->
+    lbinds L D DS ->
+    exists DS' D', binds x (μ{ DS' }) G /\ lbinds L D' DS'.
+Proof.
+  dep induction on ty_var_inv; intros;
+    eauto.
+  do 2 eexists. eroutine.
+  routine.
+Qed.
+
+(* Lemma inert_natural_obj_subtyp : forall G x DS A S U, *)
+(*     inert_env G -> *)
+(*     G ⊢## x ⦂ μ{ DS } -> *)
+(*     lbinds (label_typ A) (dec_typ S U) DS -> *)
+(*     forall DS' T, *)
+(*       binds x (μ{ DS' }) G -> *)
+(*       lbinds (label_typ A) (dec_typ T T) DS' -> *)
+(*       G ⊢# S <⦂ T /\ G ⊢# T <⦂ U. *)
+(* Proof. *)
+(*   intros G x DS A S U. intro. intro. gen S U H0. *)
+(*   dep induction on ty_var_inv; *)
+(*     intros. *)
+(*   Focus 6. *)
+(*   from_inert. *)
+(*   destruct (A == A0). subst. *)
+(*   split. apply subtypt_trans with S1. eapply H2. *)
   
+(*   list_reasoning. *)
+(*   eapply IHty_var_inv; eauto. list_reasoning. *)
+(*   repeat (apply LabelAssocList.binds_app_1 in H3; destruct H3); auto. *)
+(*   routine. *)
+
+  
+(*   eapply IHty_var_inv; eauto. list_reasoning. *)
+(*   repeat (apply LabelAssocList.binds_app_1 in H3; destruct H3); auto. *)
+(*   routine. *)
+  
+  
+(*   from_inert; auto. *)
+(*   from_inert; list_reasoning. eapply IHty_var_inv; eauto; list_reasoning; apply lbinds_app_r; auto. *)
+(*   from_inert; list_reasoning. eapply IHty_var_inv; eauto; list_reasoning; apply lbinds_app_l; auto. *)
+
+
+
+Lemma general_to_tight :
+  forall G0, inert_env G0 ->
+        (forall G t T, G ⊢ t ⦂ T ->
+                  G = G0 ->
+                  G ⊢# t ⦂ T) /\
+        (forall G S U, G ⊢ S <⦂ U ->
+                  G = G0 ->
+                  G ⊢# S <⦂ U).
+Proof.
+  mutual induction; eroutine.
+
+  recover_inert_env.
+  (* we need to prove inert_env gives a good binding *)
+  specialize (H0 eq_refl).
+
+  invert H0; eauto.
+  subst.
+  apply tight_to_invertible in H3; auto.
+  pose proof H4.
+  eapply invertible_typing_closure_tight in H5.
+  instantiate (1 := x) in H5. all:trivial.
+  apply inert_subtyp_obj in H5.
+  destruct H5.
+  from_inert.
+  
+  pose proof invertible_typing_closure_tight.
+  specialize (H5 term+)
+  
+  eauto.
+  
+  eapply subtypt_sel1.
+  
+  
+  tight typing undec 1; routine.
+  apply H1.
+  
+  eapply subtypt_all; auto.
+
+  
+  tight typing undec 1; eroutine.
+
+
+(* Hint Extern 1 => *)
+(* list_reasoning; apply lbinds_app_r. *)
+
+(* Hint Extern 1 => *)
+(* list_reasoning; apply lbinds_app_l. *)
+
+
+(* Hint Resolve lbinds_app_r. *)
+
+(* Require Import Metalib.CoqEqDec. *)
+
+(* Instance EqDec_typ_label typ_label : EqDec_eq typ_label. *)
+(* Proof. *)
+(* Admitted. *)
+
+(* Lemma inert_natural_obj_subtyp : forall G x DS A S U, *)
+(*     inert_env G -> *)
+(*     G ⊢## x ⦂ μ{ DS } -> *)
+(*     lbinds (label_typ A) (dec_typ S U) DS -> *)
+(*     forall DS' T, *)
+(*       binds x (μ{ DS' }) G -> *)
+(*       lbinds (label_typ A) (dec_typ T T) DS' -> *)
+(*       G ⊢# S <⦂ T /\ G ⊢# T <⦂ U. *)
+(* Proof. *)
+(*   intros G x DS A S U. intro. intro. gen S U H0. *)
+(*   dep induction on ty_var_inv; *)
+(*     intros. *)
+(*   Focus 6. *)
+  (* from_inert. *)
+  (* destruct (A == A0). subst. *)
+  (* split. apply subtypt_trans with S1. eapply H2. *)
+  
+  (* list_reasoning.  *)
+  (* eapply IHty_var_inv; eauto. list_reasoning. *)
+  (* repeat (apply LabelAssocList.binds_app_1 in H3; destruct H3); auto. *)
+  (* routine. *)
+
+  
+  (* eapply IHty_var_inv; eauto. list_reasoning. *)
+  (* repeat (apply LabelAssocList.binds_app_1 in H3; destruct H3); auto. *)
+  (* routine. *)
+  
+  
+  (* from_inert; auto. *)
+  (* from_inert; list_reasoning. eapply IHty_var_inv; eauto; list_reasoning; apply lbinds_app_r; auto. *)
+  (* from_inert; list_reasoning. eapply IHty_var_inv; eauto; list_reasoning; apply lbinds_app_l; auto. *)
+
+  (* from_inert. list_reasoning. *)
+  (* apply LabelAssocList.binds_app_1 in H1. *)
+  (* progressive_destructions. *)
+  (* eauto. eauto. *)
+
+  (* from_inert. eapply IHty_var_inv; eauto; list_reasoning. *)
+  (* apply LabelAssocList.binds_app_1 in H0. *)
+  (* destruct H0. eauto. *)
+  (* apply LabelAssocList.binds_app_1 in H0. *)
+  (* destruct H0. cbv in H0. routine. eauto. *)
+
+  (* from_inert. eapply IHty_var_inv. eauto. list_reasoning. *)
+  (* repeat (apply LabelAssocList.binds_app_1 in H3; destruct H3); auto. *)
+  (* routine. *)
+
+
+  
+  (* cbv in H1. destruct H1. inversion H1. subst. *)
+  (* routine. *)
+  (* routine. *)
+  
+  (* eauto. *)
+  (* change (decs_cons a (dec_trm U) DS2) with (decs_append (decs_cons a (dec_trm U) decs_nil) DS2) in H0. *)
+  (* list_reasoning. *)
+
+  
+  (* routine. *)
+  
+  (* eapply IHty_var_inv; auto. *)
+  
+
+  
+  (* from_inert_env; *)
+  (* clear_dups; from_inert_obj. *)
+
+
+  
+  (* prove from inert. *)
+
+  
+(*   progressive_destructions. *)
+(*   clear_dups. recover_inert_env. *)
+
+(*   simpl in *; cbn in *; subst. *)
+(*   autounfold in *; fold any not. *)
+  
+
+  
+(*   simplify. *)
+(*   prove from inert. *)
+  
+(*   from_inert. *)
+(*   prove from inert. *)
+
+(*     prove from inert. *)
+(*     intros. *)
+(*   from_inert_env. clear_dups. *)
+(*   match goal with *)
+(*   | [ H : inert_env ?G, H1 : binds ?x ?T1 ?G, H2 : binds ?x ?T2 ?G |- _ ] => *)
+(*     different T1 T2; *)
+(*       assert (T1 = T2); subst *)
+(*   end. *)
+(*   simplify; progressive_destructions. *)
+(*   fail_if_dup. dup_eq. *)
+(*   eapply binds_unique; eauto. *)
+  
+(*    by (fail_if_dup; dup_eq; *)
+(*                            eapply binds_unique; eassumption) *)
+  
+(*   from_inert. from_inert_env.  from_inert. clear_dups. *)
+(*   prove from inert. *)
+   
+(*     prove from inert. *)
+
+  
+(*   intros. *)
 
 
 (* Require Import Coq.Program.Equality. *)
@@ -124,38 +346,7 @@ Qed.
 (*   - left. exists DS. eapply binds_unique; routine. *)
 (*   - edestruct IHtyt_trm; try eassumption; trivial. *)
 (*     + admit. *)
-(*     + subst. right.  *)
+(*     + subst. right. *)
 (*     subst. *)
 (*   auto. *)
 (*   induction on tyt_trm. *)
-
-(* Lemma general_to_tight : *)
-(*   forall G0, inert_env G0 -> *)
-(*         (forall G t T, G ⊢ t ⦂ T -> *)
-(*                   G = G0 -> *)
-(*                   G ⊢# t ⦂ T) /\ *)
-(*         (forall G S U, G ⊢ S <⦂ U -> *)
-(*                   G = G0 -> *)
-(*                   G ⊢# S <⦂ U). *)
-(* Proof. *)
-(*   mutual induction; eroutine. *)
-
-(*   (* we need to prove inert_env gives a good binding *) *)
-(*   specialize (H0 eq_refl). *)
-
-(*   invert H0; eauto. *)
-(*   subst. *)
-
-  
-(*   eauto.  *)
-  
-(*   eapply subtypt_sel1. *)
-  
-  
-(*   tight typing undec 1; routine. *)
-(*   apply H1. *)
-  
-(*   eapply subtypt_all; auto. *)
-
-  
-(*   tight typing undec 1; eroutine. *)
